Bdd/Sim copy.lean
@@ -10,10 +10,10 @@ structure State {n m m'} (O : OBdd n m) (U : OBdd n m') where
   rl : Std.HashMap (Fin m') (Fin m)
   hl : ∀ j j',
     lr[j]? = some j' → rl[j']? = some j           ∧
-    ∃ hj hj', O.SimilarRP (U := U) ⟨.node j, hj⟩ ⟨.node j', hj'⟩
+    ∃ hj hj', OBdd.Similar (O.subBdd ⟨.node j, hj⟩) (U.subBdd ⟨.node j', hj'⟩)
   hr : ∀ j j',
     rl[j']? = some j → lr[j]? = some j'            ∧
-    ∃ hj hj', O.SimilarRP (U := U) ⟨.node j, hj⟩ ⟨.node j', hj'⟩
+    ∃ hj hj', OBdd.Similar (O.subBdd ⟨.node j, hj⟩) (U.subBdd ⟨.node j', hj'⟩)
 
 def State.insert {n m m'} {O : OBdd n m} {U : OBdd n m'} (s : State O U) (j : Fin m) (j' : Fin m')
     (hrj : Pointer.Reachable O.bdd.heap O.bdd.root (Pointer.node j))
@@ -21,8 +21,10 @@ def State.insert {n m m'} {O : OBdd n m} {U : OBdd n m'} (s : State O U) (j : Fi
     (hv : O.bdd.heap[j].var = U.bdd.heap[j'].var)
     (hl : s.lr[j]? = none)
     (hr : s.rl[j']? = none)
-    (h : OBdd.SimilarRP ⟨O.bdd.heap[j].low, .snoc hrj .low⟩ ⟨U.bdd.heap[j'].low, .snoc hrj' .low⟩)
-    (h' : OBdd.SimilarRP ⟨O.bdd.heap[j].high, .snoc hrj .high⟩ ⟨U.bdd.heap[j'].high, .snoc hrj' .high⟩)
+    (h : (O.subBdd ⟨O.bdd.heap[j].low, .snoc hrj Edge.low⟩).Similar
+      (U.subBdd ⟨U.bdd.heap[j'].low, .snoc hrj' Edge.low⟩))
+    (h' : (O.subBdd ⟨O.bdd.heap[j].high, .snoc hrj Edge.high⟩).Similar
+      (U.subBdd ⟨U.bdd.heap[j'].high, .snoc hrj' Edge.high⟩))
     : State O U where
   lr := s.lr.insert j j'
   rl := s.rl.insert j' j
@@ -37,7 +39,7 @@ def State.insert {n m m'} {O : OBdd n m} {U : OBdd n m'} (s : State O U) (j : Fi
         subst heqq
         simp only [true_and]
         use hrj, hrj'
-        simp only [OBdd.similarRP_iff] at ⊢ h h'
+        simp only [OBdd.similar_iff] at ⊢ h h'
         rw [OBdd.toTree_node (OBdd.root_subBdd ⟨.node j, _⟩)]
         rw [OBdd.toTree_node (OBdd.root_subBdd ⟨.node j', _⟩)]
         simp only [OBdd.heap_subBdd, OBdd.low_subBdd, OBdd.high_subBdd,
@@ -64,7 +66,7 @@ def State.insert {n m m'} {O : OBdd n m} {U : OBdd n m'} (s : State O U) (j : Fi
         subst heqq
         simp only [true_and]
         use hrj, hrj'
-        simp only [OBdd.similarRP_iff] at ⊢ h h'
+        simp only [OBdd.similar_iff] at ⊢ h h'
         rw [OBdd.toTree_node (OBdd.root_subBdd ⟨.node j, _⟩)]
         rw [OBdd.toTree_node (OBdd.root_subBdd ⟨.node j', _⟩)]
         simp only [OBdd.heap_subBdd, OBdd.low_subBdd, OBdd.high_subBdd,
@@ -86,20 +88,22 @@ def sim_helper {n m m'}
     (U : OBdd n m') (hU : OBdd.Reduced U)
     (p : Pointer m) (hpr : Pointer.Reachable O.1.heap O.1.root p)
     (q : Pointer m') (hqr : Pointer.Reachable U.1.heap U.1.root q) :
-    StateM (State O U) (Decidable (OBdd.SimilarRP ⟨p, hpr⟩ ⟨q, hqr⟩)) :=
+  StateM
+    (State O U)
+    (Decidable (OBdd.Similar (O.subBdd ⟨p, hpr⟩) (U.subBdd ⟨q, hqr⟩))) :=
   match hp : p with
   | .terminal b =>
     match hq : q with
     | .terminal b' =>
       if hb : b = b'
-      then return isTrue <| by simpa [OBdd.similarRP_iff, OBdd.toTree_terminal]
-      else return isFalse <| by simpa [OBdd.similarRP_iff, OBdd.toTree_terminal]
+      then return isTrue <| by simpa [OBdd.similar_iff, OBdd.toTree_terminal]
+      else return isFalse <| by simpa [OBdd.similar_iff, OBdd.toTree_terminal]
     | .node j' =>
-      return isFalse <| by simp [OBdd.similarRP_iff, OBdd.toTree_terminal, OBdd.toTree_node]
+      return isFalse <| by simp [OBdd.similar_iff, OBdd.toTree_terminal, OBdd.toTree_node]
   | .node j =>
     match hq : q with
     | .terminal b' =>
-      return isFalse <| by simp [OBdd.similarRP_iff, OBdd.toTree_terminal, OBdd.toTree_node]
+      return isFalse <| by simp [OBdd.similar_iff, OBdd.toTree_terminal, OBdd.toTree_node]
     | .node j' =>
       if hv : O.1.heap[j].var = U.1.heap[j'].var
       then do
@@ -110,15 +114,15 @@ def sim_helper {n m m'}
           | none =>
             let hll ← sim_helper O hO U hU
               O.1.heap[j].low (.snoc hpr .low) U.1.heap[j'].low (.snoc hqr .low)
-            if h : OBdd.SimilarRP ⟨O.bdd.heap[j].low, _⟩ ⟨U.bdd.heap[j'].low, _⟩ then
+            if h : (O.subBdd ⟨O.bdd.heap[j].low, _⟩).Similar (U.subBdd ⟨U.bdd.heap[j'].low, _⟩) then
               let hhh :=
                 ← sim_helper O hO U hU
                 O.1.heap[j].high (Pointer.Reachable.snoc hpr .high)
                 U.1.heap[j'].high (Pointer.Reachable.snoc hqr .high)
-              if h' : OBdd.SimilarRP ⟨O.bdd.heap[j].high, _⟩ ⟨U.bdd.heap[j'].high, _⟩ then
+              if h' : (O.subBdd ⟨O.bdd.heap[j].high, _⟩).Similar (U.subBdd ⟨U.bdd.heap[j'].high, _⟩) then
                 set (s.insert j j' hpr hqr hv hl hr h h')
                 return isTrue <| by
-                  simp only [OBdd.similarRP_iff] at ⊢ h h'
+                  simp only [OBdd.similar_iff] at ⊢ h h'
                   rw [OBdd.toTree_node (OBdd.root_subBdd ⟨.node j, _⟩)]
                   rw [OBdd.toTree_node (OBdd.root_subBdd ⟨.node j', _⟩)]
                   simp only [OBdd.heap_subBdd, OBdd.low_subBdd, OBdd.high_subBdd,
@@ -140,7 +144,7 @@ def sim_helper {n m m'}
               rcases s.hl i j' h1 with ⟨h1', h2', h3', h4'⟩
               intro contra
               have hsim : OBdd.SimilarRP ⟨.node i, h2'⟩ ⟨.node j, hpr⟩ := by
-                rw [OBdd.similarRP_iff] at contra h4
+                rw [OBdd.similar_iff] at contra h4
                 rw [OBdd.similarRP_iff, contra]
                 exact h4
               have h := hO.2 hsim
@@ -159,23 +163,23 @@ def sim_helper {n m m'}
               rcases s.hr j i' h1 with ⟨h1', h2', h3', h4'⟩
               have hsim : OBdd.SimilarRP ⟨.node j', hqr⟩ ⟨.node i', h3'⟩ := by
                 rw [OBdd.similarRP_iff]
-                rw [OBdd.similarRP_iff] at c h4
+                rw [OBdd.similar_iff] at c h4
                 rw [c] at h4
                 exact h4
               have := hU.2 hsim
               simp [InvImage] at this
               exact heq this
-      else return isFalse <| by simp_all [OBdd.similarRP_iff, OBdd.toTree_node]
+      else return isFalse <| by simp_all [OBdd.similar_iff, OBdd.toTree_node]
 termination_by OBdd.size' ⟨⟨O.1.heap, p⟩, O.ordered_of_reachable hpr⟩
 decreasing_by
   · simp [OBdd.size'_node, OBdd.low_eq, Bdd.low_eq]; omega
   · simp [OBdd.size'_node, OBdd.high_eq, Bdd.high_eq]; omega
 
-public def decidableRobddSimilar {n m m'}
+public def decidableRobddHSimilar {n m m'}
     (O : OBdd n m) (hO : O.Reduced)
     (U : OBdd n m') (hU : U.Reduced) :
     Decidable (O.Similar U) :=
-  @decidable_of_iff' _ _ OBdd.similar_iff_similarRP
+  O.subBdd_root ▸ U.subBdd_root ▸
     (sim_helper O hO U hU O.1.root .refl U.1.root .refl ⟨∅, ∅, by simp, by simp⟩).1
 
 end Sim
